Make k in orderedBitvec a parameter, Axiom K_ge1 captures that k must be positive, no other assumption needed

Isa/Val.v
@@ -1,4 +1,4 @@
-Require Import Util EqDec List bitvec.
+Require Import Arith Util EqDec List bitvec.
 Require Import OrderedTypeEx.
 
 Set Implicit Arguments.
@@ -8,14 +8,14 @@ Set Implicit Arguments.
 
 (** Make the value type bitvectors and the default value 0 as a bitvector **)
 Definition val := bitvec.
-Definition default_val : val := (zext k (O::nil)).
+Definition default_val : val := (zext (O::nil)).
 
 Opaque val.
 Opaque default_val.
 
 (** Default value for true = 1 = 2^1 , false = 0 = 2^0 **)
-Definition val_true := (zext k (I::nil)).
-Definition val_false := (zext k (O::nil)).
+Definition val_true := (sext (I::nil) I).
+Definition val_false := (zext (O::nil)).
 
 Fixpoint eqValList (l1:list bitvec) (l2:list bitvec) :=
 match l1, l2 with
@@ -45,13 +45,16 @@ Definition val2bool : val -> bool := fun v => toBool  v. (*  match v with 0 => f
 Lemma val2bool_true
 : val2bool val_true = true.
 Proof.
-  reflexivity.
+  unfold val_true, val2bool, sext.
+  rewrite toBool_I_true; [auto|].
+  pose proof K_ge1; auto.
 Qed.
 
 Lemma val2bool_false
 : val2bool val_false = false.
 Proof.
-  reflexivity.
+  unfold val2bool, val_false, zext.
+  rewrite toBool_O_false; auto.
 Qed.
 
 Opaque val2bool.
